@prefix rdf: <http://www.w3.org/1999/02/22-rdf-syntax-ns#> .
@prefix rdfs: <http://www.w3.org/2000/01/rdf-schema#> .
@prefix owl: <http://www.w3.org/2002/07/owl#> .
@prefix xsd: <http://www.w3.org/2001/XMLSchema#> .
@prefix skos: <http://www.w3.org/2004/02/skos/core#> .
@prefix dcterms: <http://purl.org/dc/terms/> .
@prefix foaf: <http://xmlns.com/foaf/0.1/>.
@prefix vann: <http://purl.org/vocab/vann/> .
@prefix voaf: <http://purl.org/vocommons/voaf#> .
@prefix time: <http://www.w3.org/2006/time#> .
@prefix prov: <https://www.w3.org/TR/prov-o/#> .
@prefix doap: <http://usefulinc.com/ns/doap#> .

@prefix schema: <http://schema.org/> .

@prefix ogc: <http://www.opengis.net/def/ont/modspec/> . 
@prefix sosa: <http://www.w3.org/ns/sosa/> .
@prefix sosa-oms: <http://www.w3.org/ns/sosa/oms> .

dcterms:title a owl:AnnotationProperty .
dcterms:description a owl:AnnotationProperty .
dcterms:rights a owl:AnnotationProperty .
dcterms:license a owl:AnnotationProperty .
dcterms:created a owl:AnnotationProperty .
dcterms:creator a owl:AnnotationProperty .
foaf:Agent a owl:Class .
foaf:name a owl:AnnotationProperty .
schema:domainIncludes a owl:AnnotationProperty .
schema:rangeIncludes a owl:AnnotationProperty .
skos:definition a owl:AnnotationProperty .
skos:example a owl:AnnotationProperty .
skos:note a owl:AnnotationProperty .
time:TemporalEntity a owl:Class .
vann:preferredNamespacePrefix a owl:AnnotationProperty .
vann:preferredNamespaceUri a owl:AnnotationProperty .
voaf:Vocabulary a owl:Class .


sosa-oms: a owl:Ontology ;
  dcterms:title "OMS Ontology - based on (SOSA) Ontology"@en ;
  dcterms:description "This ontology is based on the SOSA Ontology by the W3C/OGC Spatial Data on the Web Working Group, supplemented by some classes and properties required to implement ISO 19156:2023 ."@en ;
  dcterms:creator [ a foaf:Agent ; foaf:name "W3C/OGC Spatial Data on the Web Working Group"@en ] ;
  dcterms:rights "Copyright 2024 W3C/OGC." ;
  dcterms:license <http://www.w3.org/Consortium/Legal/2015/copyright-software-and-document> ;
  dcterms:license <http://www.opengeospatial.org/ogc/Software> ;
  dcterms:created "2023-10-07"^^xsd:date ;
  dcterms:source <https://docs.ogc.org/as/20-082r4/20-082r4.html> ;
  rdfs:comment "The original source of each resource is indicated by the rdfs:isDefinedBy property" ;
  owl:imports sosa: .

ogc:implements a owl:ObjectProperty ;
    skos:definition "link from an RDFS/OWL class or property to a requirement linked to an element in a UML model which it implements" ;
    rdfs:subPropertyOf dcterms:source , prov:wasDerivedFrom , doap:implements . 

## General properties

sosa:metadata a owl:OjectProperty ;
  ogc:implements <http://www.opengis.net/spec/om/3.0/req/obs-core/gen/metadata-sem> ;
  schema:domainIncludes sosa:FeatureOfInterest ,
                        sosa:ObservableProperty ,
                        sosa:Observation ,
                        sosa:ObservationCollection , 
                        sosa:Sample ,
                        sosa:SampleCollection ,
                        sosa:Sampling ,
                        sosa:PreparationStep ,
                        sosa:Procedure ,
                        sosa:Sensor ,
                        sosa:Platform ,
                        sosa:Deployment ; 
    rdfs:isDefinedBy sosa-oms: .


## Features of interest and Property
## largely defined in ISO 19103 and ISO 19109

sosa:FeatureOfInterest 
  rdfs:isDefinedBy sosa: .

sosa:ObservableProperty ogc:implements <http://www.opengis.net/spec/om/3.0/req/obs-cpt/ObservableProperty> ;
    rdfs:subClassOf sosa:Property ;
    rdfs:isDefinedBy sosa: .

sosa:ActuatableProperty 
    rdfs:subClassOf sosa:Property ;
    rdfs:isDefinedBy sosa: .

sosa:Property 
  rdfs:isDefinedBy sosa: .

sosa:hasProperty 
    owl:inverseOf sosa:isPropertyOf ;
    rdfs:isDefinedBy sosa: .

sosa:isPropertyOf 
    owl:inverseOf sosa:hasProperty ; 
    rdfs:isDefinedBy sosa: .

## Sample 

sosa:Sample ogc:implements <http://www.opengis.net/spec/om/3.0/req/sam-cpt/Sample> ;
  rdfs:subClassOf sosa:FeatureOfInterest ;
  rdfs:subClassOf sosa:Result ; 
  rdfs:isDefinedBy sosa: .

sosa:hasSample 
    owl:inverseOf sosa:isSampleOf ;
    rdfs:isDefinedBy sosa: .

sosa:isSampleOf ogc:implements <http://www.opengis.net/spec/om/3.0/req/sam-cpt/Sample/sampledFeature-sem> ;
    owl:inverseOf sosa:hasSample ;
    rdfs:isDefinedBy sosa: .

sosa:hasOriginalSample 
  rdfs:isDefinedBy sosa: .

sosa:hasSampledFeature ogc:implements <http://www.opengis.net/spec/om/3.0/req/sam-cpt/Sample/sampledFeature-sem> ;
  rdfs:isDefinedBy sosa: .

sosa:hasPreparationStep a owl:ObjectProperty ;
  ogc:implements <http://www.opengis.net/spec/om/3.0/req/sam-cpt/Sample/preparationStep-sem> ;
  rdfs:label "has preparation step"@en ;
  skos:definition "Link to a preparation step used to prepare the sample"@en ;
  rdfs:comment "Link to a preparation step used to prepare the sample"@en ;
  schema:domainIncludes sosa:Sample ;
  schema:rangeIncludes sosa:PreparationStep ;
  rdfs:isDefinedBy sosa-oms: .

sosa:SpatialSample a rdfs:Class , owl:Class ;
  ogc:implements <http://www.opengis.net/spec/om/3.0/req/sam-basic/SpatialSample> ;
  rdfs:subClassOf sosa:Sample ; 
  rdfs:label "Spatial Sample"@en ;
  skos:definition "A SpatialSample is a geospatial Sample. When observations are made to estimate properties of a geospatial feature, in particular where the value of a property varies within the scope of the feature, a SpatialSample is used."@en ;
  rdfs:comment "A SpatialSample is a geospatial Sample. When observations are made to estimate properties of a geospatial feature, in particular where the value of a property varies within the scope of the feature, a SpatialSample is used."@en ;
  skos:example "Some common names for spatial samples include: borehole, flightline, interval, lidar cloud, map horizon, microscope slide, mine level, mine, observation well, profile, pulp, quadrat, scene, section, ship track, spot, station, swath, trajectory, traverse, etc..."@en ;
  skos:note "Depending on accessibility and on the nature of the expected property variation, the SpatialSample may be extensive in one, two or three spatial dimensions."@en ;
  rdfs:isDefinedBy sosa-oms: .

sosa:MaterialSample a rdfs:Class , owl:Class ;
  ogc:implements <http://www.opengis.net/spec/om/3.0/req/sam-basic/MaterialSample> ;
  rdfs:subClassOf sosa:Sample ; 
  rdfs:label "Material Sample"@en ;
  skos:definition "A MaterialSample is a physical, tangible Sample."@en ;
  rdfs:comment "A MaterialSample is a physical, tangible Sample."@en ;
  skos:example "A piece of rock, a blood sample, a water sample, etc."@en ;
  skos:note "MaterialSamples that are curated and preserved are sometimes known as 'specimens'."@en ;
  skos:note "MaterialSamples may be destroyed in connexion with the observation act or a subsequent preparation step."@en ;
  rdfs:isDefinedBy sosa-oms: .

sosa:StatisticalSample a rdfs:Class , owl:Class ;
  ogc:implements <http://www.opengis.net/spec/om/3.0/req/sam-basic/StatisticalSample> ;
  rdfs:subClassOf sosa:Sample ; 
  rdfs:label "Statistical Sample"@en ;
  skos:definition "A StatisticalSample is a statistical subset of a feature-of-interest, defined for the purpose of creating Observation(s)."@en ;
  rdfs:comment "A StatisticalSample is a statistical subset of a feature-of-interest, defined for the purpose of creating Observation(s)."@en ;
  skos:example "The male or female subset of a population."@en ;
  skos:note "StatisticalSamples usually apply to populations or other sets, of which certain subset may be of specific interest."@en ;
  rdfs:isDefinedBy sosa-oms: .

sosa:SampleCollection ogc:implements <http://www.opengis.net/spec/om/3.0/req/sam-basic/SampleCollection> ;
  rdfs:isDefinedBy sosa: .

sosa:hasMemberSample ogc:implements <http://www.opengis.net/spec/om/3.0/req/sam-basic/SampleCollection/member-sem> ;
  rdfs:subPropertyOf rdfs:member ;
  rdfs:isDefinedBy sosa: .

## Platform 

sosa:Platform ogc:implements <http://www.opengis.net/spec/om/3.0/req/obs-cpt/Host> ;
  rdfs:subClassOf sosa:System ;
  rdfs:isDefinedBy sosa: .

sosa:hosts ogc:implements <http://www.opengis.net/spec/om/3.0/req/obs-cpt/gen/relatedObservation-sem> ;
  owl:inverseOf sosa:isHostedBy ;
  rdfs:isDefinedBy sosa: .

sosa:isHostedBy ogc:implements <http://www.opengis.net/spec/om/3.0/req/obs-cpt/Observation/host-sem> ;
  owl:inverseOf sosa:hosts ;
  rdfs:isDefinedBy sosa: .


## Procedures

sosa:Procedure ogc:implements <http://www.opengis.net/spec/om/3.0/req/obs-cpt/Procedure> ;
  rdfs:isDefinedBy sosa: .

sosa:ObservingProcedure a rdfs:Class , owl:Class ;
  ogc:implements <http://www.opengis.net/spec/om/3.0/req/obs-cpt/ObservingProcedure> ;
  rdfs:subClassOf sosa:Procedure ;  
  rdfs:label "Observing Procedure"@en ;
  skos:definition "The description of steps performed in order to determine the value of an ObservableProperty by an Observer."@en ;
  rdfs:comment "The description of steps performed in order to determine the value of an ObservableProperty by an Observer."@en ;
  skos:example "A workflow, protocol, plan, algorithm, or computational method specifying how to make an observation; the description of the process utilized by an observer. This could be a chemical analysis method, a protocol for measuring an object, but could also be a checklist utilized by a human observer during a biodiversity campaign."@en ;
  skos:note "The observing procedure cannot describe a sensor instance, but it can describe the sensor type."@en ;
  rdfs:isDefinedBy sosa-oms: .

sosa:ActuationProcedure a rdfs:Class , owl:Class ;
  rdfs:subClassOf sosa:Procedure ;
  rdfs:label "Actuation Procedure"@en ;
  skos:definition "The description of steps performed by an Actuator to change the ActuableProperty."@en ;
  rdfs:comment "The description of steps performed by an Actuator to change the ActuableProperty."@en ;
  rdfs:isDefinedBy sosa-oms: .

sosa:SamplingProcedure a rdfs:Class , owl:Class ;
  ogc:implements <http://www.opengis.net/spec/om/3.0/req/sam-cpt/SamplingProcedure> ;
  rdfs:subClassOf sosa:Procedure ;
  rdfs:label "Sampling Procedure"@en ;
  skos:definition "The description of steps performed by a Sampler in order to extract a Sample from its sampled Feature in the frame of a Sampling."@en ;
  rdfs:comment "The description of steps performed by a Sampler in order to extract a Sample from its sampled Feature in the frame of a Sampling."@en ;
  rdfs:isDefinedBy sosa-oms: .

sosa:PreparationProcedure a rdfs:Class , owl:Class ;
  ogc:implements <http://www.opengis.net/spec/om/3.0/req/sam-cpt/PreparationProcedure> ;
  rdfs:subClassOf sosa:Procedure ;
  rdfs:label "Preparation Procedure"@en ;
  skos:definition "The description of preparation steps performed on a Sample."@en ;
  rdfs:comment "The description of preparation steps performed on a Sample."@en ;
  rdfs:isDefinedBy sosa-oms: .


## ProcedureExecutors

sosa:Sensor ogc:implements <http://www.opengis.net/spec/om/3.0/req/obs-cpt/Observer> ;
  rdfs:subClassOf sosa:System ;
  rdfs:isDefinedBy sosa: .

  sosa:observes ogc:implements <http://www.opengis.net/spec/om/3.0/req/obs-cpt/Observer/observableProperty-sem> ;
    rdfs:subPropertyOf sosa:forProperty ;
    owl:inverseOf sosa:isObservedBy ;
    rdfs:isDefinedBy sosa: .

  sosa:isObservedBy ogc:implements <http://www.opengis.net/spec/om/3.0/req/obs-cpt/ObservableProperty/observer-sem> ;
    owl:inverseOf sosa:observes ;
    rdfs:isDefinedBy sosa: .

sosa:Sampler ogc:implements <http://www.opengis.net/spec/om/3.0/req/sam-cpt/Sampler> ;
  rdfs:subClassOf sosa:System ;
  rdfs:isDefinedBy sosa: .

sosa:implements  ogc:implements <http://www.opengis.net/spec/om/3.0/req/obs-cpt/Observer/observingProcedure-sem>  ,
                                <http://www.opengis.net/spec/om/3.0/req/sam-cpt/Sampling/samplingProcedure-sem> ;
  owl:inverseOf sosa:implementedBy ;
  rdfs:isDefinedBy sosa: .

sosa:implementedBy ogc:implements <http://www.opengis.net/spec/om/3.0/req/obs-cpt/ObservingProcedure/observer-sem> ,
                                  <http://www.opengis.net/spec/om/3.0/req/sam-cpt/SamplingProcedure/sampler-sem> ;
  owl:inverseOf sosa:implements ;
  rdfs:isDefinedBy sosa: .


## ProcedureExecutions

sosa:usedProcedure ogc:implements <http://www.opengis.net/spec/om/3.0/req/obs-cpt/Observation/observingProcedure-sem> ,
                                  <http://www.opengis.net/spec/om/3.0/req/sam-cpt/Sampling/samplingProcedure-sem> ;
  rdfs:isDefinedBy sosa: .

sosa:hasFeatureOfInterest ogc:implements <http://www.opengis.net/spec/om/3.0/req/obs-cpt/Observation/featureOfInterest-sem> 
                                , <http://www.opengis.net/spec/om/3.0/req/obs-core/AbstractObservationCharacteristics/pFoI-sem> 
                                , <http://www.opengis.net/spec/om/3.0/req/sam-cpt/Sampling/featureOfInterest-sem>;
  owl:inverseOf sosa:isFeatureOfInterestOf ;
  rdfs:isDefinedBy sosa: .

sosa:hasUltimateFeatureOfInterest ogc:implements <http://www.opengis.net/spec/om/3.0/req/obs-core/AbstractObservationCharacteristics/uFoI-sem> ;
  rdfs:isDefinedBy sosa: .

sosa:isFeatureOfInterestOf 
  ogc:implements <http://www.opengis.net/spec/om/3.0/req/obs-cpt/gen/relatedObservation-sem> ;
  owl:inverseOf sosa:hasFeatureOfInterest ;
  rdfs:isDefinedBy sosa: .

sosa:Observation ogc:implements <http://www.opengis.net/spec/om/3.0/req/obs-cpt/Observation> ;
  rdfs:isDefinedBy sosa: .

  sosa:madeObservation ogc:implements <http://www.opengis.net/spec/om/3.0/req/obs-cpt/gen/relatedObservation-sem> ;
    owl:inverseOf sosa:madeBySensor ;
    rdfs:isDefinedBy sosa: .

  sosa:madeBySensor ogc:implements <http://www.opengis.net/spec/om/3.0/req/obs-cpt/Observation/observer-sem> ;
    owl:inverseOf sosa:madeObservation ;
    rdfs:isDefinedBy sosa: .

  sosa:observedProperty ogc:implements <http://www.opengis.net/spec/om/3.0/req/obs-cpt/Observation/observedProperty-sem> ;
    rdfs:isDefinedBy sosa: .

  sosa:madeOnPlatform rdf:type owl:ObjectProperty ;
    ogc:implements <http://www.opengis.net/spec/om/3.0/req/obs-cpt/Observation/host-sem> ;
    rdfs:label "made on platform"@en ;
    skos:definition "Relation between an Observation and the Platform the Sensor was attached to at the time the observation was made."@en ;
    rdfs:comment "Relation between an Observation and the Platform the Sensor was attached to at the time the observation was made."@en ;
    schema:domainIncludes sosa:Observation ;
    schema:domainIncludes sosa:ObservationCollection ;
    schema:rangeIncludes sosa:Platform ;
    rdfs:isDefinedBy sosa-oms: .

  sosa:relatedObservation rdf:type owl:ObjectProperty ;
    ogc:implements <http://www.opengis.net/spec/om/3.0/req/obs-cpt/gen/relatedObservation-sem> ;
    rdfs:label "related observation"@en ;
    skos:definition "Relation to an Observation."@en ;
    rdfs:comment "Relation to an Observation."@en ;
    schema:domainIncludes sosa:Sample ;
    schema:domainIncludes sosa:ObservableProperty ;
    schema:domainIncludes sosa:ObservingProcedure ;
    schema:domainIncludes sosa:Sensor ;
    schema:domainIncludes sosa:Platform ;
    schema:domainIncludes osa:Observation ;
    schema:domainIncludes sosa:ObservationCollection ;
    schema:rangeIncludes sosa:Observation ;
    rdfs:isDefinedBy sosa-oms: .

sosa:Sampling ogc:implements <http://www.opengis.net/spec/om/3.0/req/sam-cpt/Sampling> ;
  rdfs:isDefinedBy sosa: .

  sosa:madeSampling ogc:implements <http://www.opengis.net/spec/om/3.0/req/sam-cpt/Sampler/sampling-sem> ;
    owl:inverseOf sosa:madeBySampler ;
    rdfs:isDefinedBy sosa: .

  sosa:madeBySampler ogc:implements <http://www.opengis.net/spec/om/3.0/req/sam-cpt/Sampling/sampler-sem> ;
    owl:inverseOf sosa:madeSampling ;
    rdfs:isDefinedBy sosa: .

  sosa:relatedSampling rdf:type owl:ObjectProperty ;
    ogc:implements <http://www.opengis.net/spec/om/3.0/req/sam-cpt/Sampling/relatedSampling-sem> ;
    rdfs:label "related sampling"@en ;
    skos:definition "Relation to an act of Sampling."@en ;
    rdfs:comment "Relation to an act of Sampling."@en ;
    schema:domainIncludes sosa:Sampling ;
    schema:rangeIncludes sosa:Sampling ;
    rdfs:isDefinedBy sosa-oms: .

sosa:PreparationStep a rdfs:Class , owl:Class ;
  ogc:implements <http://www.opengis.net/spec/om/3.0/req/sam-cpt/PreparationStep> ;
  rdfs:label "Preparation Step"@en ;
  skos:definition "A PreparationStep is an individual step pertaining to a Sample PreparationProcedure."@en ;
  rdfs:comment "A PreparationStep is an individual step pertaining to a Sample PreparationProcedure."@en ;
  skos:example "???"@en ;
  rdfs:isDefinedBy sosa-oms: .

  sosa:preparedSample a owl:ObjectProperty ;
    ogc:implements <http://www.opengis.net/spec/om/3.0/req/sam-cpt/PreparationStep/preparedSample-sem> ;
    rdfs:label "prepared sample"@en ;
    skos:definition "The Sample on which the PreparationProcedure is performed."@en ;
    rdfs:comment "The Sample on which the PreparationProcedure is performed."@en ;
    schema:domainIncludes sosa:PreparationStep ;
    schema:rangeIncludes sosa:Sample ;
    rdfs:isDefinedBy sosa-oms: .

  sosa:processingDetails a owl:ObjectProperty ;
    ogc:implements <http://www.opengis.net/spec/om/3.0/req/sam-cpt/PreparationStep/processingDetails-sem> ;
    rdfs:label "processing details"@en ;
    skos:definition "The PreparationProcedure used by the PreparationStep."@en ;
    rdfs:comment "The PreparationProcedure used by the PreparationStep."@en ;
    schema:domainIncludes sosa:PreparationStep ;
    schema:rangeIncludes sosa:PreparationProcedure ;
    rdfs:isDefinedBy sosa-oms: .

  sosa:samplePreparationStep a owl:ObjectProperty ;
    ogc:implements <http://www.opengis.net/spec/om/3.0/req/sam-cpt/PreparationProcedure/samplePreparationStep-sem> ;
    rdfs:label "sample preparation step"@en ;
    skos:definition "A PreparationStep that uses the PreparationProcedure."@en ;
    rdfs:comment "A PreparationStep that uses the PreparationProcedure."@en ;
    schema:domainIncludes sosa:PreparationProcedure ;
    schema:rangeIncludes sosa:PreparationStep ;
    rdfs:isDefinedBy sosa-oms: .


## Observation Collection

sosa:ObservationCollection ogc:implements <http://www.opengis.net/spec/om/3.0/req/obs-core/AbstractObservationCollection> ;
  rdfs:isDefinedBy sosa: .

sosa:hasMemberObs ogc:implements <http://www.opengis.net/spec/om/3.0/req/obs-core/AbstractObservationCollection/member-sem> ;
  rdfs:subPropertyOf rdfs:member ;
  rdfs:isDefinedBy sosa: .


## Result 

sosa:Result 
  rdfs:isDefinedBy sosa: .

  sosa:hasResult ogc:implements <http://www.opengis.net/spec/om/3.0/req/obs-cpt/Observation/result-sem> ,
                                <http://www.opengis.net/spec/om/3.0/req/sam-cpt/Sampling/result-sem>;
    owl:inverseOf sosa:isResultOf ;
    rdfs:isDefinedBy sosa: .

  sosa:isResultOf 
    ogc:implements <http://www.opengis.net/spec/om/3.0/req/obs-cpt/gen/relatedObservation-sem> ;
    owl:inverseOf sosa:hasResult ;
    rdfs:isDefinedBy sosa: .

  sosa:hasSimpleResult ogc:implements <http://www.opengis.net/spec/om/3.0/req/obs-cpt/Observation/result-sem> ;
    rdfs:isDefinedBy sosa: .

  # for sampling

#  sosa:hasResultingSample a owl:ObjectProperty ;
#    rdfs:label "has resulting sample"@en ;
#    skos:definition "Relation linking an act of Sampling and the new Sample created as a result."@en ;
#    rdfs:comment "Relation linking an act of Sampling and the new Sample created as a result."@en ;
#    schema:domainIncludes sosa:Sampling ;
#    schema:rangeIncludes sosa:Sample ;
#    owl:inverseOf sosa:isSamplingResultOf ;
#    rdfs:isDefinedBy sosa: .

#  sosa:isSamplingResultOf a owl:ObjectProperty ;
#    rdfs:label "is sampling result of"@en ;
#    skos:definition "Relation linking a Sample to the act of Sampling that created or caused it."@en ;
#    rdfs:comment "Relation linking a Sample to the act of Sampling that created or caused it."@en ;
#    schema:domainIncludes sosa:Sample ;
#    schema:rangeIncludes sosa:Sampling ;
#    owl:inverseOf sosa:hasResultingSample ;
#    rdfs:isDefinedBy sosa: .


sosa:resultTime ogc:implements <http://www.opengis.net/spec/om/3.0/req/obs-cpt/Observation/resultTime-sem> ;
  rdfs:isDefinedBy sosa: .

sosa:phenomenonTime ogc:implements <http://www.opengis.net/spec/om/3.0/req/obs-cpt/Observation/phenomenonTime-sem> ;
  rdfs:isDefinedBy sosa: .

sosa:validTime a owl:ObjectProperty ;
  ogc:implements <http://www.opengis.net/spec/om/3.0/req/obs-cpt/Observation/validTime-sem> ;
  rdfs:label "valid time"@en ;
  skos:definition "The time interval during which the result is assumed to be applicable for use."@en ;
  rdfs:comment "The time interval during which the result is assumed to be applicable for use."@en ;
  schema:domainIncludes sosa:Actuation ;
  schema:domainIncludes sosa:Observation ;
  schema:domainIncludes sosa:Sampling ;
  schema:rangeIncludes time:Interval , dcterms:PeriodOfTime ;
  rdfs:isDefinedBy sosa-oms: .


## Deployment

sosa:Deployment ogc:implements <http://www.opengis.net/spec/om/3.0/req/obs-cpt/Deployment> ;
  rdfs:isDefinedBy sosa: .

  sosa:deployedOnPlatform ogc:implements <http://www.opengis.net/spec/om/3.0/req/obs-cpt/Deployment/host-sem> ;
    owl:inverseOf sosa:inDeployment ;
    rdfs:isDefinedBy sosa: .

  sosa:deployedSystem ogc:implements <http://www.opengis.net/spec/om/3.0/req/obs-cpt/Deployment/observer-sem> ;
    rdfs:subPropertyOf sosa:deployedAsset ;
    owl:inverseOf sosa:hasDeployment ;
    rdfs:isDefinedBy sosa: .

  sosa:hasDeployment ogc:implements <http://www.opengis.net/spec/om/3.0/req/obs-cpt/Observer/deployment-sem> ;
    owl:inverseOf sosa:deployedSystem ;
    rdfs:isDefinedBy sosa: .

  sosa:inDeployment ogc:implements <http://www.opengis.net/spec/om/3.0/req/obs-cpt/Host/deployment-sem> ;
    owl:inverseOf sosa:deployedOnPlatform ;
    rdfs:isDefinedBy sosa: .

